Test/Peano.lean
@@ -1,8 +1,54 @@
-import Zag.Theory
+import Lib.Peano.Defs
 
 namespace Zag
 
-def PrimitiveCtx.Peano : PrimitiveCtx :=
-  [
-    ("Nat", Nat)
+private abbrev comparisonCtx : PrimitiveCtx :=
+  .ofPrims [
+    .of "Nat" Nat,
+    .of "Bool" Bool
   ]
+
+private instance : Peano.Types comparisonCtx where
+  natType := by rfl
+  boolType := by rfl
+
+private def optionNat (value : Option Nat) : Val comparisonCtx :=
+  .mk (.option Peano.NatTy) (cast (by
+    rw [Ty.type.eq_3, Ty.type.eq_2, Peano.Types.natType]
+    rfl : Option Nat = Ty.type comparisonCtx (.option Peano.NatTy)) value)
+
+example : Val.primEq? (Val.nat (primCtx := comparisonCtx) 0) (Val.bool false) = none := by
+  have hboolNat : (Val.bool (primCtx := comparisonCtx) false).asNat? = none := by
+    simp only [Val.asNat?, Val.bool, Val.as?]
+    simp
+  have hnatBool : (Val.nat (primCtx := comparisonCtx) 0).asBool? = none := by
+    simp only [Val.asBool?, Val.nat, Val.as?]
+    simp
+  simp [Val.primEq?, hboolNat, hnatBool]
+
+example : Val.primLt? (Val.bool (primCtx := comparisonCtx) false) (Val.nat 1) = none := by
+  have hboolNat : (Val.bool (primCtx := comparisonCtx) false).asNat? = none := by
+    simp only [Val.asNat?, Val.bool, Val.as?]
+    simp
+  have hnatBool : (Val.nat (primCtx := comparisonCtx) 1).asBool? = none := by
+    simp only [Val.asBool?, Val.nat, Val.as?]
+    simp
+  simp [Val.primLt?, hboolNat, hnatBool]
+
+example :
+    (Op.compare (primCtx := comparisonCtx) Val.primEq?).out
+      (fun i : Fin 2 => if i = 0 then Peano.NatTy else Peano.BoolTy) = none := by
+  simp [Op.compare]
+
+example :
+    Op.applyVals (Op.compare Val.primEq?)
+      [optionNat none, optionNat (some 1)] = none := by
+  simp [Op.applyVals, Op.compare, Op.Body.applyVals, optionNat, Val.primEq?, Val.asNat?,
+    Val.asBool?, Val.as?]
+
+example :
+    Op.applyVals (Op.compare (primCtx := comparisonCtx) (fun _ _ => none))
+      [Val.nat 1, Val.nat 1] = none := by
+  simp [Op.applyVals, Op.compare, Op.Body.applyVals]
+
+end Zag
