Test/Gauss.lean
@@ -1,2 +1,4 @@
 import Test.Gauss.Rec
 import Test.Gauss.SSA
+import Test.Monad
+import Test.Peano
